Poe/Examples/First.lean
@@ -78,14 +78,14 @@ def testInts : List Int := (List.range 11).map fun n => Int.ofNat n - 5
 def testLists : List (List Int) := [[], [1], [1, 2, 3], [-3, -2, -1, 0, 1, 2, 3], [5, 5, 5]]
 
 #eval show Lean.CoreM Unit from
-  Poe.Oracle.runSuite ``double (testInts.map fun x => ([Poe.Oracle.encodeInt x], double x))
+  Poe.Oracle.runSuite ``double (testInts.map fun x => ([Poe.Oracle.encodeInt x], .integer (double x)))
 
 #eval show Lean.CoreM Unit from
-  Poe.Oracle.runSuite ``absInt (testInts.map fun x => ([Poe.Oracle.encodeInt x], absInt x))
+  Poe.Oracle.runSuite ``absInt (testInts.map fun x => ([Poe.Oracle.encodeInt x], .integer (absInt x)))
 
 #eval show Lean.CoreM Unit from do
   let cases ← testLists.mapM fun xs => do
-    return ([← Poe.Oracle.encodeIntList xs], sumList xs)
+    return ([← Poe.Oracle.encodeIntList xs], .integer (sumList xs))
   Poe.Oracle.runSuite ``sumList cases
 
 end Poe.Examples
